SepLogic.thy
@@ -320,6 +320,9 @@ subsection \<open> Seplogic connectives \<close>
 definition sepconj :: \<open>('a \<Rightarrow> bool) \<Rightarrow> ('a \<Rightarrow> bool) \<Rightarrow> ('a \<Rightarrow> bool)\<close> (infixl \<open>\<^emph>\<close> 88) where
   \<open>P \<^emph> Q \<equiv> \<lambda>h. \<exists>h1 h2. h1 ## h2 \<and> h = h1 + h2 \<and> P h1 \<and> Q h2\<close>
 
+lemma sepconj_iff: \<open>(P \<^emph> Q) r = (\<exists>h1 h2. h1 ## h2 \<and> r = h1 + h2 \<and> P h1 \<and> Q h2)\<close>
+  by (simp add: sepconj_def)
+
 definition sepimp :: \<open>('a \<Rightarrow> bool) \<Rightarrow> ('a \<Rightarrow> bool) \<Rightarrow> ('a \<Rightarrow> bool)\<close> (infixr \<open>\<midarrow>\<^emph>\<close> 65) where
   \<open>P \<midarrow>\<^emph> Q \<equiv> \<lambda>h. \<forall>h1. h ## h1 \<longrightarrow> P h1 \<longrightarrow> Q (h + h1)\<close>
 
